src/SubstSemantics.v
@@ -6,25 +6,6 @@ Require Export FSets.FMapFacts. *)
 
 Import ListNotations.
 
-Ltac break_match_hyp :=
-match goal with
-| [ H : context [ match ?X with _=>_ end ] |- _] =>
-     match type of X with
-     | sumbool _ _=>destruct X
-     | _=>destruct X eqn:? 
-     end 
-end.
-
-Ltac break_match_goal :=
-match goal with
-| [ |- context [ match ?X with _=>_ end ] ] => 
-    match type of X with
-    | sumbool _ _ => destruct X
-    | _ => destruct X eqn:?
-    end
-end.
-
-
 Inductive is_value : Exp -> Prop :=
 | ELit_val : forall l, is_value (ELit l)
 | EFun_val : forall vl e, is_value (EFun vl e)
@@ -35,130 +16,6 @@ Inductive ResultType {T : Set} : Set :=
 | Fail
 | Res (v : T)
 .
-
-(* The equality of function signatures *)
-Definition funid_eqb (v1 v2 : FunctionIdentifier) : bool :=
-match v1, v2 with
-| (fid1, num1), (fid2, num2) => String.eqb fid1 fid2 && Nat.eqb num1 num2
-end.
-
-(* Extended equality between functions and vars *)
-Definition var_funid_eqb (v1 v2 : Var + FunctionIdentifier) : bool :=
-match v1, v2 with
-| inl s1, inl s2 => String.eqb s1 s2
-| inr f1, inr f2 => funid_eqb f1 f2
-| _, _ => false
-end.
-
-  Proposition funid_eqb_eq (f f' : FunctionIdentifier):
-    funid_eqb f f' = true <-> f = f'.
-  Proof.
-    intuition.
-    * destruct f, f'. simpl in H. apply Bool.andb_true_iff in H. destruct H.
-      apply eqb_eq in H. apply Nat.eqb_eq in H0. subst. reflexivity.
-    * subst. destruct f'. simpl. rewrite eqb_refl, Nat.eqb_refl. auto.
-  Qed.
-
-  Proposition funid_eqb_neq (f f0 : FunctionIdentifier):
-    funid_eqb f f0 = false <-> f <> f0.
-  Proof.
-    intuition.
-    * destruct f, f0. simpl in H. apply Bool.andb_false_iff in H. inversion H.
-        - apply eqb_neq in H1. unfold not in *. apply H1. inversion H0. reflexivity.
-        - apply Nat.eqb_neq in H1. unfold not in *. apply H1. inversion H0. reflexivity.
-    * simpl. destruct f, f0. simpl. apply Bool.andb_false_iff.
-        unfold not in H. case_eq ((s =? s0)%string); intros.
-        - right. apply eqb_eq in H0. apply Nat.eqb_neq. unfold not. intro. apply H. subst. reflexivity.
-        - left. reflexivity.
-  Qed.
-
-  Proposition var_funid_eqb_eq (v0 v : Var + FunctionIdentifier):
-    var_funid_eqb v0 v = true <-> v0 = v.
-  Proof.
-    intros. split; intros.
-    { destruct v0, v.
-      * inversion H. apply eqb_eq in H1. subst. reflexivity.
-      * inversion H.
-      * inversion H.
-      * apply funid_eqb_eq in H. subst. auto.
-    }
-    { destruct v, v0.
-      * inversion H. subst. simpl. apply eqb_refl.
-      * inversion H.
-      * inversion H.
-      * simpl. apply funid_eqb_eq. inversion H. auto.
-    }
-  Qed.
-
-  Proposition var_funid_eqb_neq (v0 v : Var + FunctionIdentifier):
-    var_funid_eqb v0 v = false <-> v0 <> v.
-  Proof.
-    split; intros.
-    { destruct v0, v.
-      * simpl in *. apply eqb_neq in H. unfold not in *. intros. apply H. inversion H0. reflexivity.
-      * unfold not. intro. inversion H0.
-      * unfold not. intro. inversion H0.
-      * apply funid_eqb_neq in H. intro. congruence.
-    }
-    { destruct v0, v.
-      * simpl in *. apply eqb_neq. unfold not in *. intro. apply H. subst. reflexivity.
-      * simpl. reflexivity.
-      * simpl. reflexivity.
-      * apply funid_eqb_neq. intro. congruence.
-    }
-  Qed.
-
-  Proposition funid_eqb_refl (f : FunctionIdentifier) :
-    funid_eqb f f = true.
-  Proof.
-    destruct f. simpl. simpl. rewrite eqb_refl, Nat.eqb_refl. simpl. reflexivity.
-  Qed.
-
-  Proposition var_funid_eqb_refl (var : Var + FunctionIdentifier) :
-    var_funid_eqb var var = true.
-  Proof.
-    destruct var.
-    * simpl. apply eqb_refl.
-    * destruct f. simpl. rewrite eqb_refl, Nat.eqb_refl. simpl. reflexivity.
-  Qed.
-
-Fixpoint varsubst (v' : Var) (what wher : Exp) : Exp :=
-match wher with
- | ELit l => wher
- | EVar v => if String.eqb v v' then what else EVar v
- | EFunId f => wher
- | EFun vl e => if in_list v' vl then EFun vl e else EFun vl (varsubst v' what e)
- | ERecFun f vl e => if in_list v' vl then ERecFun f vl e else ERecFun f vl (varsubst v' what e)
- | EApp exp l => EApp (varsubst v' what exp) (map (varsubst v' what) l)
- | ELet v e1 e2 => if String.eqb v v' then ELet v (varsubst v' what e1) e2
-                               else ELet v (varsubst v' what e1) (varsubst v' what e2)
- | ELetRec f vl b e => if in_list v' vl then ELetRec f vl b (varsubst v' what e) 
-                                        else ELetRec f vl (varsubst v' what b) (varsubst v' what e)
- | EPlus e1 e2 => EPlus (varsubst v' what e1) (varsubst v' what e2)
- | EIf e1 e2 e3 => EIf (varsubst v' what e1) (varsubst v' what e2) (varsubst v' what e3) 
-end.
-
-Fixpoint funsubst (f' : FunctionIdentifier) (what wher : Exp) : Exp :=
-match wher with
- | ELit l => wher
- | EVar v => EVar v
- | EFunId f => if funid_eqb f f' then what else wher
- | EFun vl e => EFun vl (funsubst f' what e)
- | ERecFun f vl e => if funid_eqb f f' 
-                     then ERecFun f vl e
-                     else ERecFun f vl (funsubst f' what e)
- | EApp exp l => EApp (funsubst f' what exp) (map (funsubst f' what) l)
- | ELet v e1 e2 => ELet v (funsubst f' what e1) (funsubst f' what e2)
- | ELetRec f vl b e => if funid_eqb f f'
-                       then ELetRec f vl b e
-                       else ELetRec f vl (funsubst f' what b) (funsubst f' what e)
- | EPlus e1 e2 => EPlus (funsubst f' what e1) (funsubst f' what e2)
- | EIf e1 e2 e3 => EIf (funsubst f' what e1) (funsubst f' what e2) (funsubst f' what e3)
-end.
-
-
-Definition varsubst_list (l : list Var) (es : list Exp) (e : Exp) : Exp :=
-  fold_right (fun '(v, val) acc => varsubst v val acc) e (combine l es).
 
 Inductive list_forall {A : Type} (P : A -> Prop) : list A -> Prop :=
 | forall_nil : list_forall P []
@@ -196,7 +53,7 @@ match clock with
                                match vres with
                                | Res vals => 
                                  if length vals =? length vl
-                                 then eval n (varsubst_list vl vals e)
+                                 then eval n (subst (idsubst[[::= combine (map inl vl) vals]]) e)
                                  else Fail
                                | Fail => Fail
                                | Timeout => Timeout
@@ -206,7 +63,7 @@ match clock with
                                match vres with
                                | Res vals => 
                                  if length vals =? length vl
-                                 then eval n (varsubst_list vl vals (funsubst f (ERecFun f vl e) e))
+                                 then eval n (subst (idsubst[[::= (inr f, ERecFun f vl e) :: combine (map inl vl) vals]]) e)
                                  else Fail
                                | Fail => Fail
                                | Timeout => Timeout
@@ -215,10 +72,10 @@ match clock with
                          | r => r
                          end
          | ELet v e1 e2 => match eval n e1 with
-                           | Res val => eval n (varsubst v val e2)
+                           | Res val => eval n (subst (idsubst[[inl v ::= val]]) e2)
                            | r      => r
                            end
-         | ELetRec f vl b e => eval n (funsubst f (ERecFun f vl b) e)
+         | ELetRec f vl b e => eval n (subst (idsubst[[inr f ::= ERecFun f vl b]]) e)
          | EPlus e1 e2 => 
             match eval n e1, eval n e2 with
             | Res (ELit n), Res (ELit m) => Res (ELit (n + m))
@@ -234,6 +91,12 @@ match clock with
             end
         end
 end.
+
+Goal eval 10 (inc 2) = Res (ELit 3). Proof. auto. Qed.
+Goal eval 10 (simplefun 10) = Res (ELit 10). Proof. simpl. auto. Qed.
+Goal eval 10 (sum 2) = Res (ELit 3). Proof. simpl. auto. Qed.
+Goal eval 100 (sum 10) = Res (ELit 55). Proof. simpl. auto. Qed.
+Goal eval 100 (simplefun2 10 10) = Res (ELit 20). Proof. simpl. auto. Qed.
 
 Theorem indexed_to_forall {A : Type} (l : list A) : forall P def,
   list_forall P l
